% Custom semantic coloring
\newcommand{\A}[1]{\textcolor{purple}{#1}}          % Elements from A
\newcommand{\B}[1]{\textcolor{orange!80!black}{#1}} % Elements from B
\newcommand{\F}[1]{\textcolor{blue!60!black}{#1}}   % Scalars from F

\begin{technical}
{\Large\textbf{Two Equivalences of the Exponential Map}}\\[0.4em]

\noindent\textbf{Functional Characterization via Derivation Operator}\\[0.3em]

Let \( \A{A} \) be an additive group and \( \B{B} \) a unital algebra over a field \( \F{F} \). Let \( \mathrm{Func}(\A{A}, \B{B}) \) denote the algebra of functions from \( \A{A} \) to \( \B{B} \), equipped with pointwise operations inherited from \( \B{B} \). Suppose there exists a linear operator
\[
K: \mathrm{Func}(\A{A}, \B{B}) \to \mathrm{Func}(\A{A}, \B{B})
\]
satisfying for all \( g, h \in \mathrm{Func}(\A{A}, \B{B}) \), and all \( \F{c} \in \F{F} \):
(i) Linearity: \( K(g + h) = K(g) + K(h) \), \( K(\F{c} \cdot g) = \F{c} \cdot K(g) \);
(ii) Product Rule: \( K(g \cdot h) = K(g) \cdot h + g \cdot K(h) \);
(iii) Kills Constants: \( K(c_{\B{b}}) = \B{0} \), where \( c_{\B{b}}(\A{x}) \equiv \B{b} \in \B{B} \).

Let \( f \in \mathrm{Func}(\A{A}, \B{B}) \) satisfy:
(iv) \( K(f) = \F{\lambda} \cdot f \);
(v) \( f(\A{0}) = \B{1} \);
(vi) For all \( \A{y} \in \A{A} \), define \( g_{\A{y}}(\A{x}) := f(\A{x} \A{+} \A{y}) \), and assume \( K(g_{\A{y}}) = \F{\lambda} \cdot g_{\A{y}} \);
(vii) If \( K(g) = \F{\lambda} \cdot g \) and \( g(\A{0}) = \B{0} \), then \( g(\A{x}) = \B{0} \) for all \( \A{x} \).

Define the function \( g(\A{x}) := f(\A{x} \A{+} \A{y}) - f(\A{x}) \B{\cdot} f(\A{y}) \).
\begin{align*}
g(\A{0}) 
&= f(\A{y}) - f(\A{0}) \B{\cdot} f(\A{y}) \\
&= f(\A{y}) - \B{1} \B{\cdot} f(\A{y}) \\
&= \B{0}.
\end{align*}

Now compute \( K(g) \), using linearity and the product rule:
\begin{align*}
K(g)(\A{x}) 
&= K\big(f(\A{x} \A{+} \A{y})\big) - K\big(f(\A{x}) \B{\cdot} f(\A{y})\big) \\
&= \F{\lambda} \cdot f(\A{x} \A{+} \A{y}) - \Big( K(f(\A{x})) \B{\cdot} f(\A{y}) + f(\A{x}) \B{\cdot} K(f(\A{y})) \Big) \\
&= \F{\lambda} \cdot f(\A{x} \A{+} \A{y}) - \Big( \F{\lambda} \cdot f(\A{x}) \B{\cdot} f(\A{y}) + \F{\lambda} \cdot f(\A{x}) \B{\cdot} f(\A{y}) \Big) \\
&= \F{\lambda} \cdot f(\A{x} \A{+} \A{y}) - 2 \F{\lambda} \cdot f(\A{x}) \B{\cdot} f(\A{y}) \\
&= \F{\lambda} \cdot \left( f(\A{x} \A{+} \A{y}) - f(\A{x}) \B{\cdot} f(\A{y}) \right) \\
&= \F{\lambda} \cdot g(\A{x}).
\end{align*}

So \( K(g) = \F{\lambda} \cdot g \), and since \( g(\A{0}) = \B{0} \), uniqueness (vii) implies \( g(\A{x}) = \B{0} \) for all \( \A{x} \). Hence:
\[
f(\A{x} \A{+} \A{y}) = f(\A{x}) \B{\cdot} f(\A{y}).
\]

This confirms that the exponential law emerges directly from the derivation structure, normalization, and shift invariance — independent of analytic assumptions.

\vspace{0.5em}

\noindent\textbf{Geometric Interpretation in Riemannian Manifolds}\\[0.3em]

Let \( M \) be a Riemannian manifold and \( p \in M \). The exponential map at \( p \) is defined as \( \exp_p(v) := \gamma_v(1) \), where \( \gamma_v \) is the geodesic starting at \( p \) with velocity \( v \), solving:
\( \frac{D}{dt} \dot{\gamma}_v(t) = 0 \), \( \gamma_v(0) = p \), \( \dot{\gamma}_v(0) = v \).

In \( \mathbb{R}^n \), geodesics are straight lines: \( \gamma_v(t) = p + tv \), so \( \exp_p(v) = p + v \).

In a Lie group \( G \subset \mathrm{GL}_n(\mathbb{R}) \): \( \gamma_X(t) = \exp(tX) \) satisfies \( \frac{d}{dt}\gamma(t) = X\gamma(t) \), \( \gamma(0) = I \).

This mirrors the scalar case: \( x'(t) = ax(t) \), \( x(0) = 1 \) yields \( x(t) = e^{at} \).

The exponential map lifts linear generators — derivations or tangent vectors — to integrated flows across groups or manifolds, justifying its name in both analytic and geometric settings.

\vspace{0.3em}
\noindent\textbf{References:}\\
Lang, S. (2001). \textit{Fundamentals of Differential Geometry}. Springer.\\
Kobayashi, S., \& Nomizu, K. (1963). \textit{Foundations of Differential Geometry, Vol. I}. Wiley.
\end{technical}
